fv: refactor circuit instances

fv/crates/lean_extraction/src/instance.rs
@@ -1,0 +1,57 @@
+use core::marker::PhantomData;
+
+use ff::Field;
+use ragu_core::convert::WireMap;
+use ragu_core::gadgets::Gadget;
+
+use crate::driver::ExtractionDriver;
+use crate::expr::Expr;
+
+/// A [`WireMap`] that collects all physical wires from a gadget by cloning
+/// them into a flat [`Vec`].
+///
+/// Used by [`CircuitInstance`] implementors to manually serialize the output
+/// of a circuit into a list of driver wires.
+pub struct WireCollector<F: Field> {
+    pub wires: Vec<Expr<F>>,
+}
+
+impl<F: Field> WireCollector<F> {
+    pub fn new() -> Self {
+        WireCollector { wires: Vec::new() }
+    }
+
+    pub fn collect_from<'dr, G>(gadget: &G) -> ragu_core::Result<Vec<Expr<F>>>
+    where
+        G: Gadget<'dr, ExtractionDriver<F>>,
+        ExtractionDriver<F>: ragu_core::drivers::Driver<'dr, F = F>,
+    {
+        let mut collector = Self::new();
+        gadget.map(&mut collector)?;
+        Ok(collector.wires)
+    }
+}
+
+impl<F: Field> WireMap<F> for WireCollector<F> {
+    type Src = ExtractionDriver<F>;
+    type Dst = PhantomData<F>;
+
+    fn convert_wire(&mut self, wire: &Expr<F>) -> ragu_core::Result<()> {
+        self.wires.push(wire.clone());
+        Ok(())
+    }
+}
+
+/// A trait for circuit instances that can be extracted by the driver.
+pub trait CircuitInstance {
+    type Field: Field + std::fmt::Debug;
+
+    /// Run the circuit on `dr` and return its output.
+    /// The output is a vector of expressions corresponding to the
+    /// output wires in order. This must include all "interesting" wires for which we
+    /// want to prove some properties about.
+    /// They have to be physical wires (i.e. `Expr::Var`) since virtual wires cannot be
+    /// referenced from outside the circuit.
+    fn circuit(dr: &mut ExtractionDriver<Self::Field>)
+    -> ragu_core::Result<Vec<Expr<Self::Field>>>;
+}
